thys/MRBNF_Recursor.thy
@@ -300,8 +300,8 @@ ML_file \<open>../Tools/mrbnf_sugar.ML\<close>
 
 (*ML_file \<open>../Tools/binder_inductive.ML\<close>*)
 
-context begin
+(*context begin
 ML_file \<open>../Tools/binder_induction.ML\<close>
-end
+end*)
 
 end
